# CSDS 133 Written Homework 3
**Instructions:** Each question is worth 10 points unless otherwise stated. Write your answers below the question. Only one answer is needed from a group unless otherwise specified. Each answer should be formatted so it renders properly on github. **Answers that do not render properly may not be graded.** Each person in each group must commit and push their own work. You will not get credit for work committed/pushed by someone else even if done by you. Each person is expected to do an approximately equal share of the work, as shown by the git logs. **If we do not see evidence of equal contribution from the logs for someone, their individual grade will be reduced substantially.** Please comment the last commit with "FINAL COMMIT" and **enter the final commit ID in canvas by the due date.**

Note: Questions which ask you to "prove" something often require a general argument rather than specific examples. For other questions, please show your work rather than just the final answer for full credit.

1. Find $f \circ g$ and $g \circ f$ for $f(x)=\sqrt{(x+2)}$ and $g(x)=\frac{1}{x}$.

Answer: f o g = f(1/x) = sqrt((1/x) + 2) , g o f = g(sqrt(x+2)) = 1/sqrt(x+2)

2. Using the definition of the derivative, show that $\frac{d}{dx}\frac{1}{x}=\frac{-1}{x^2}$. 

Answer: limit as h approaches 0 = (1/(x+h) - 1/x)/h = -1/((x+h)(x)) = -1/x^2


3. Prove the quotient rule using the product rule and the chain rule of derivatives. You can use the result from Q2 above.

Answer: 
Quotient Rule: (f(x)/g(x))' = (f'(x)g(x) - f(x)g'(x))/g(x)^2

Product Rule = (f(x)g(x))' = f(x)g'(x) + g(x)f'(x)

Chain Rule = (f(g(x)))' = f'(g(x))(g'(x))
        
Proof using the product rule and chain rule:
        
        1. Rewrite the quotient rule as a product of two functions
        (f(x)/g(x))' = (f(x)/g(x)) * (g'(x)/g(x)')
        
        2. By using the chaine rule, we can calculate the derivative of the second factor (g'(x)/g(x))
        (g'(x)/g(x)) = (-g'(x)/g(x)^2) * g'(x) + (1/g(x)) * g''(x)) = (-g'(x)/g(x)^2) * g'(x) + (1/g(x)) * g''(x) = (-g''(x)/g(x)) + (g'(x)/g(x))^2
        
        3. Now, substitute the simplified expression from above back into the original equation
        (f(x)/g(x))' = (f(x)/g(x)) * ((-g''(x)/g(x)) + (g'(x)/g(x))^2)
        
        4. Finally, by applying the product rule to the right hand side of the equation above, we are left with the quotient rule.
        (f(x)/g(x))' = (f'(x)g(x))/g(x) - f(x)g'(x))/g(x)^2
        (f(x)/g(x))' = (f'(x)g(x) - f(x)g'(x))/g(x)^2
        
        

4. Find the derivative of $f(x)=a^x$ where $a$ is a constant. Show your work. (Hint: Write $f(x)$ as an exponential function and use the chain rule.)

Answer: 

f(x) as an exponential function: f(x) = e^(x * ln(a))

f'(x) = e^(x * ln(a) * d/dx(x * ln(a)))

d/dx(x * ln(a)) = x * d/dx(ln(a)) + ln(a) * d/dx(x) = ln(a)

f'(x) = e^(x * ln(a)) * ln(a), a^x = e^(x * ln(a)) => f'(x) = a^(x * ln(a))


5.  Find the Jacobian of $f(x,y)=\[x^y, y^x, e^{xy}\]$. Show your work. (Hint: The derivative of $x^n$, $n$ constant, is $nx^{n-1}$.)

Answer: 

           | x^(y-1) * y  ,  (x^y) * ln(x) |
           | y^x * ln(y)  ,  y^(x-1) * x   |
           | e^(xy) * y  ,  e^(yx) * x     |

6. Let $f(x, y, z)=(x^2+z, x+y^2)$. Let $g(a, b)=(a^3b^2, a^2b^3, a^2−b^3)$. Find the Jacobian of $f \circ g$. Show your work.

Answer: 


f(a^3 * b^2, a^2 * b^3, a^2-b^3) = (a^6 * b^4 + a^2-b^3, a^3 * b^2 + a^4 * b^6)


| 6(a^5 * b^4) + 2a  ,  4(b^3 * a^6) - 3b^2                 |


| 4(a^3 * b^6) + 3(a^2 * b^2)  ,  6(b^5 * a^4) + 2(b * a^3) |



7. Find the Hessian of $f \circ g$ from Q6. Show your work.

Answer: 


f(a^3 * b^2, a^2 * b^3, a^2-b^3) = (a^6 * b^4 + a^2-b^3, a^3 * b^2 + a^4 * b^6)


df/da = ( 6(a^5 * b^4) + 2a  ,  3(a^2 * b^2) + 4(a^3 * b^6) )


df/db = ( 4(a^6 * b^3) - 3b^2  ,  2(a^3 * b) + 6(a^4 * b^5) )


| { 30(a^4 * b^4) + 2  ,  12(a^6 * b^6) + 6(a * b^2) }  ,  { 24(b^3 * a^5)  ,  24(b^5 * a^3) + 6(b^2 * a) } |


| { 24(a^5 * b^3)  ,  24(a^3 * b^5) + 6(a^2 * b) }  ,  { 12(b^2 * a^6) - 6b  ,  30(b^4 * a^4) + 2a^3 }      |




8. Prof. Calculus is climbing Mt. Steepy McSteepface. At each point $(x,y)$ the mountain has height $h(x,y)= 100e^{-(x^2+y^2-6x-8y+25)}$. Help Prof. Calculus by finding the height of the summit. Show your work.

Answer:

Take partial derivatives of $h(x, y)$.

$∂h/∂x = -200(x-3)e^{-(x^2+y^2-6x-8y+25)}$

$∂h/∂y = -200(y-4)e^{-(x^2+y^2-6x-8y+25)}$

Set equations to 0 and solve for system of equations for x and y.

$-200(x-3)e^{-(x^2+y^2-6x-8y+25)} = 0$

$-200(y-4)e^{-(x^2+y^2-6x-8y+25)} = 0$

x = 3, y = 4

Plug values of x and y into $h(x, y)$ to get height of the summit.

$h(3,4) = 100e^{-((3)^2+(4)^2-6(3)-8(4)+25)} = 100$ units

9. When Prof. Calculus reaches the point on the mountain with $(x,y)$ coordinates of $(2, 2)$ in Q8 they feel an urgent need to return to the base camp which is at $(0,0)$. Find the best direction they should start to move in at this point to return quickly to camp. 

Answer:
Find the gradient of the function $h(x,y)$ at point (2,2) which will gives us the vector that points in the direction of the steepest ascent of the mountain at that point.

$grad(h(x,y)) = (∂h/∂x, ∂h/∂y)$

Use the partial derivatives found in Q8 with values (2,2).

$∂h/∂x = -200((2)-3)e^{-((2)^2+(2)^2-6(2)-8(2)+25)} = 1.348$

$∂h/∂y = -200((2)-4)e^{-((2)^2+(2)^2-6(2)-8(2)+25)} = 2.695$

$grad(h(2,2)) = (1.348,2.695)$

To return to camp, you must move in the opposite direction of the gradient vector. In addition, you can normalize this vector by dividing by its magnitude.

$(-1.348,-2.695)$

$||(-1.348,-2.695)|| = sqrt((-1.348)^2 + (-2.695)^2) = 3.013$

$(-1.348/3.013,-2.695/3.013)$

$(-0.447,-0.894)$

Prof Calculus should move in the direction $(-0.447, -0.894)$ from point $(2,2)$ to retrun to base camp at point $(0,0)$.

10. Show that the set $C=\\{x : Ax \geq b\\}$ , with $A$ a matrix of size $(m,n)$, $x$ a vector of size $n$, $b$ a vector of size $m$, is a convex set. 

Answer:

For $C={x: Ax \geq b}$ to be a convex set, we need to prove that for any two points $x_1, x_2 \in C$, the line segment connecting them, the set ${tx_1 + (1-t)x_2 : 0 \leq t \leq 1}$, is also in $C$.

Let $x_1, x_2 \in C$ be two points.

$Ax_1 \geq b$ and $Ax_2 \geq b$
 
Show that for any $0 \leq t \leq 1$, the point $tx_1 + (1-t)x_2$ is also in $C$.
 
$A(tx_1 + (1-t)x_2) \geq b$

$tAx_1 + (1-t)Ax_2 \geq b$

Since $Ax_1 \geq b$ and $Ax_2 \geq b$, we have $tAx_1 \geq tb$ and $(1-t)Ax_2 \geq (1-t)b$. Add these inequalities.

$tAx_1 + (1-t)Ax_2 \geq tb + (1-t)b = b$

$A(tx_1 + (1-t)x_2) \geq b$

The point $tx_1 + (1-t)x_2$ is also in $C$. For any $x_1, x_2 \in C$ and any $0 \leq t \leq 1$, $C$ is a convex set.

11. Suppose $S=\\{x : \Vert x\Vert \leq 1\\}$ where $x$ are vectors of size $n$. Show that $S$ is a convex set.

Answer: 

For $S={x : |x| \leq 1}$ to be a convex set, we need to prove that for any two points $x_1, x_2 \in S$, the line segment connecting them, the set ${tx_1 + (1-t)x_2 : 0 \leq t \leq 1}$, is also in $S$.

Let $x_1, x_2 \in S$ be two points.

$|x_1| \leq 1$ and $|x_2| \leq 1$

Show that for any $0 \leq t \leq 1$, the point $tx_1 + (1-t)x_2$ is also in $S$.

$|tx_1 + (1-t)x_2| \leq 1$.

Use the triangle inequality for the norm, which says that $|a + b| \leq |a| + |b|$ for any vectors $a$ and $b$.

$|tx_1 + (1-t)x_2| \leq |tx_1| + |(1-t)x_2| = t|x_1| + (1-t)|x_2| \leq t + (1-t) = 1$

$|tx_1 + (1-t)x_2| \leq 1$

The point $tx_1 + (1-t)x_2$ is also in $S$. For any $x_1, x_2 \in S$ and any $0 \leq t \leq 1$, $S$ is a convex set.

12. Suppose $f$ and $g$ are two arbitrary convex functions. Prove or give a counterexample: (i) $f+g$ is convex (ii) $f-g$ is convex.

Answer: 

(i) To prove that $f+g$ is convex, we need to prove that for any two points $x_1, x_2 \in f+g$, the line segment connecting them, the set ${tx_1 + (1-t)x_2 : 0 \leq t \leq 1}$, is also in $f+g$.

$(f+g)(tx_1 + (1-t)x_2) = f(tx_1 + (1-t)x_2) + g(tx_1 + (1-t)x_2) \leq t(f+g)(x_1) + (1-t)(f+g)(x_2)$

This inequality holds for all convex $f$ and $g$, so $f+g$ is convex.

(ii) To prove that $f-g$ is convex, we need to prove that for any two points $x_1, x_2 \in f+g$, the line segment connecting them, the set ${tx_1 + (1-t)x_2 : 0 \leq t \leq 1}$, is also in $f-g$.

$(f-g)(tx_1 + (1-t)x_2) = f(tx_1 + (1-t)x_2) - g(tx_1 + (1-t)x_2) \leq t(f-g)(x_1) + (1-t)(f-g)(x_2)$

This inequality doesn't hold for all convex $f$ and $g$, so $f-g$ is not always convex.

Counterexample: Let $f(x) = x$ and $g(x) = -x$. Both $f$ and $g$ are convex, since they are both straight lines with slope $1$ and $-1$.

Since $(f-g)(0) = 0$ and $(f-g)(1) = 2$, $(f-g)(x) = 2x$ is not convex. The line connecting these points is above the graph of $f-g$ on $0 \leq t \leq 1$.





